no message

execution/examples/Dexter2FA12.v
@@ -1,4 +1,4 @@
-From Coq Require Import ZArith.
+From Coq Require Import ZArith Bool.
 From Coq Require Import Morphisms.
 Require Import Monads.
 Require Import Extras.
@@ -226,7 +226,7 @@ Definition receive (chain : Chain) (ctx : ContractCallContext)
   let sender := ctx.(ctx_from) in
   let without_actions := option_map (fun new_state => (new_state, [])) in
   let without_statechange acts := Some (state, acts) in
-  if ctx.(ctx_amount) >? 0
+  if 0 <? ctx.(ctx_amount)
   then None (* DontSendTez *)
   else match maybe_msg with
   | Some (msg_transfer param) => without_actions (try_transfer sender param state)
@@ -239,4 +239,670 @@ Definition receive (chain : Chain) (ctx : ContractCallContext)
   end.
 Close Scope Z_scope.
 
+Definition contract : Contract Setup Msg State :=
+  build_contract init receive.
+
+
+
+Section Theories.
+
+(* receive only returns Some if the sender amount is zero *)
+Lemma contract_not_payable : forall prev_state new_state chain ctx msg new_acts,
+  receive chain ctx prev_state msg = Some (new_state, new_acts) ->
+    ((ctx_amount ctx) <= 0)%Z.
+Proof.
+  intros * receive_some.
+  unfold receive in receive_some.
+  destruct_match eqn:amount in receive_some.
+  - (* case: ctx_amount > 0 *)
+    congruence.
+  - (* case: ctx_amount <= 0 *)
+    now rewrite Z.ltb_ge in amount.
+Qed.
+
+Lemma contract_not_payable' : forall prev_state chain ctx msg,
+  (0 < (ctx_amount ctx))%Z ->
+    receive chain ctx prev_state msg = None.
+Proof.
+  intros * ctx_amount_positive.
+  unfold receive.
+  destruct_match eqn:amount.
+  - (* case: ctx_amount > 0 *)
+    reflexivity.
+  - (* case: ctx_amount <= 0 *)
+    now apply Z.ltb_ge in amount.
+Qed.
+
+Ltac receive_simpl_step :=
+  match goal with
+  | H : receive _ _ _ _ = Some (_, _) |- _ =>
+      apply contract_not_payable in H as ctx_amount_zero;
+      apply Z.ltb_ge in ctx_amount_zero;
+      unfold receive in H;
+      rewrite ctx_amount_zero in H;
+      cbn in H
+  | |- receive _ _ _ _ = _ =>
+      unfold receive; cbn
+  | H : Some _ = Some _ |- _ =>
+      inversion_clear H
+  | H : Some _ = None |- _ =>
+      inversion H
+  | H : None = Some _ |- _ =>
+      inversion H
+  | H : returnIf _ = None |- _ =>
+    let G := fresh "G" in
+      unfold returnIf in H;
+      destruct_match eqn:G in H; try congruence;
+      clear H;
+      rename G into H
+  | H : returnIf _ = Some ?u |- _ =>
+    let G := fresh "G" in
+      unfold returnIf in H;
+      destruct_match eqn:G in H; try congruence;
+      clear H u;
+      rename G into H
+  | H : option_map (fun s : State => (s, _)) match ?m with | Some _ => _ | None => None end = Some _ |- _ =>
+    let a := fresh "H" in
+    destruct m eqn:a in H; try setoid_rewrite a; cbn in *; try congruence
+  | H : option_map (fun s : State => (s, _)) (if ?m then ?a else ?b) = Some _ |- _ =>
+    match a with
+    | None =>
+      let a := fresh "H" in
+      destruct m eqn:a in H; try setoid_rewrite a; cbn in *; try congruence
+    | _ => match b with
+           | None =>
+             let a := fresh "H" in
+             destruct m eqn:a in H; try setoid_rewrite a; cbn in *; try congruence
+           | _ => idtac
+    end end
+  | H : (if ?m then ?a else ?b) = Some _ |- _ =>
+    match a with
+    | None =>
+      let a := fresh "H" in
+      destruct m eqn:a in H; try setoid_rewrite a; cbn in *; try congruence
+    | _ => match b with
+           | None =>
+             let a := fresh "H" in
+             destruct m eqn:a in H; try setoid_rewrite a; cbn in *; try congruence
+           | _ => idtac
+    end end
+  end.
+(*
+  | H : context[receive] |- _ => unfold receive in H
+  | |- context[receive] => unfold receive
+  | H : context[Blockchain.receive] |- _ => unfold Blockchain.receive; cbn in H
+  | H : context[try_transfer] |- _ => unfold try_transfer in H
+  | H : context[try_transfer_from] |- _ => unfold try_transfer_from in H
+  | H : context[try_approve] |- _ => unfold try_approve in H
+  | |- context[Blockchain.receive] => unfold Blockchain.receive; cbn
+  | |- context[try_transfer] => unfold try_transfer
+  | |- context[try_transfer_from] => unfold try_transfer_from
+  | |- context[try_approve] => unfold try_approve
+*)
+
+Tactic Notation "receive_simpl" := repeat receive_simpl_step.
+
+
+
+(* ------------------- Admin is constant ------------------- *)
+
+(* admin cannot be changed *)
+Lemma admin_constant : forall prev_state new_state chain ctx new_acts msg,
+  receive chain ctx prev_state msg = Some (new_state, new_acts) ->
+    admin prev_state = admin new_state.
+Proof.
+  intros * receive_some.
+  receive_simpl.
+  destruct msg. destruct m.
+  all : now receive_simpl.
+Qed.
+
+
+
+(* ------------------- Default entrypoint correct ------------------- *)
+
+(* Default entrypoint should never succeed *)
+Lemma default_entrypoint_none : forall prev_state chain ctx,
+  receive chain ctx prev_state None = None.
+Proof.
+  intros *.
+  receive_simpl.
+  now destruct_match.
+Qed.
+
+
+
+(* ------------------- Transfer correct ------------------- *)
+
+Definition transfer_balance_update_correct old_state new_state from to amount :=
+  let get_balance addr state := with_default 0 (FMap.find addr state.(tokens)) in
+  let from_balance_before := get_balance from old_state in
+  let to_balance_before := get_balance to old_state in
+  let from_balance_after := get_balance from new_state in
+  let to_balance_after := get_balance to new_state in
+  (* if the transfer is a self-transfer, balances should remain unchained *)
+  if address_eqb from to
+  then
+    (from_balance_before =? from_balance_after) &&
+    (to_balance_before =? to_balance_after)
+  else
+    (from_balance_before =? from_balance_after + amount) &&
+    (to_balance_before + amount =? to_balance_after).
+
+(* try_transfer correctly moves <amount> from <from> to <to> *)
+Lemma try_transfer_balance_correct : forall prev_state new_state chain ctx new_acts param,
+  receive chain ctx prev_state (Some (msg_transfer param)) = Some (new_state, new_acts) ->
+  transfer_balance_update_correct prev_state new_state param.(from) param.(to) param.(value) = true.
+Proof.
+  intros * receive_some.
+  receive_simpl.
+  rename H1 into enough_balance.
+  rewrite N.ltb_ge in enough_balance.
+  unfold transfer_balance_update_correct.
+  cbn.
+  destruct_match eqn:from_to_eqb.
+  - (* from = to *)
+    destruct (address_eqb_spec param.(from) param.(to)) as [<-|]; auto.
+    rewrite !FMap.find_add.
+    cbn.
+    rewrite !N.sub_add; auto.
+    now setoid_rewrite N.eqb_refl.
+  - (* from <> to *)
+    destruct (address_eqb_spec param.(from) param.(to)) as [| from_to_eq]; auto.
+    rewrite FMap.find_add_ne; auto.
+    rewrite ?FMap.find_add.
+    rewrite FMap.find_add_ne; auto.
+    cbn.
+    rewrite !N.sub_add; auto.
+    now setoid_rewrite N.eqb_refl.
+Qed.
+
+Definition transfer_allowances_update_correct old_state new_state sender from amount :=
+  let get_allowance addr1 addr2 state := with_default 0 (FMap.find (addr1, addr2) state.(allowances)) in
+  let allowance_before := get_allowance from sender old_state in
+  let allowance_after := get_allowance from sender new_state in
+  (* if the from and sender is equal, allowances should remain unchained *)
+  if address_eqb sender from
+  then
+    (allowance_before =? allowance_after)
+  else
+    (allowance_before =? allowance_after + amount).
+
+(* try_transfer correctly subtracts <amount> from allowances if <sender> is not <from> *)
+Lemma try_transfer_allowance_correct : forall prev_state new_state chain ctx new_acts param,
+  receive chain ctx prev_state (Some (msg_transfer param)) = Some (new_state, new_acts) ->
+  transfer_allowances_update_correct prev_state new_state ctx.(ctx_from) param.(from) param.(value) = true.
+Proof.
+  intros * receive_some.
+  receive_simpl.
+  clear g0 H1.
+  unfold transfer_allowances_update_correct.
+  cbn.
+  destruct_match eqn:sender_from_eqb.
+  - (* sender = from *)
+    rename H into allowances_eq.
+    inversion_clear allowances_eq.
+    now rewrite N.eqb_refl.
+  - (* sender <> from *)
+    receive_simpl.
+    rename H0 into enough_allowance.
+    rewrite N.ltb_ge in enough_allowance.
+    rewrite FMap.find_add.
+    cbn.
+    rewrite N.sub_add; auto.
+    now rewrite N.eqb_refl.
+Qed.
+
+(* try_transfer does not produce any new actions *)
+Lemma try_transfer_new_acts_correct : forall prev_state new_state chain ctx new_acts param,
+  receive chain ctx prev_state (Some (msg_transfer param)) = Some (new_state, new_acts) ->
+    new_acts = [].
+Proof.
+  intros * receive_some.
+  receive_simpl.
+Qed.
+
+(* try_transfer does not change the total supply of tokens *)
+Lemma try_transfer_preserves_total_supply : forall prev_state new_state chain ctx new_acts param,
+  receive chain ctx prev_state (Some (msg_transfer param)) = Some (new_state, new_acts) ->
+    total_supply prev_state = total_supply new_state.
+Proof.
+  intros * receive_some.
+  receive_simpl.
+Qed.
+
+(* try_transfer only modifies the <from> and <to> balances *)
+Lemma try_transfer_preserves_other_balances : forall prev_state new_state chain ctx new_acts param,
+  receive chain ctx prev_state (Some (msg_transfer param)) = Some (new_state, new_acts) ->
+    forall account, account <> param.(from) -> account <> param.(to) ->
+      FMap.find account (tokens prev_state) = FMap.find account (tokens new_state).
+Proof.
+  intros * receive_some account account_not_from account_not_to.
+  receive_simpl.
+  cbn.
+  rewrite !FMap.find_add_ne; auto.
+Qed.
+
+(* try_transfer only modifies the <sender> and <from> allowances *)
+Lemma try_transfer_preserves_other_allowances : forall prev_state new_state chain ctx new_acts param,
+  receive chain ctx prev_state (Some (msg_transfer param)) = Some (new_state, new_acts) ->
+    forall allowance_key, allowance_key <> (param.(from), ctx.(ctx_from)) ->
+      FMap.find allowance_key (allowances prev_state) = FMap.find allowance_key (allowances new_state).
+Proof.
+  intros * receive_some account allowance_key_ne.
+  receive_simpl.
+  cbn.
+  rename H into allowance_eq.
+  destruct_address_eq.
+  - (* from = sender *)
+    now inversion_clear allowance_eq.
+  - (* from <> sender *)
+    destruct_match in allowance_eq;
+      inversion_clear allowance_eq;
+      rewrite !FMap.find_add_ne; auto.
+Qed.
+
+(* If the requirements are met then then receive on transfer msg must succeed and
+    if receive on transfer msg succeeds then requirements must hold *)
+Lemma try_transfer_is_some : forall state chain ctx param,
+  (ctx_amount ctx <= 0)%Z /\
+  param.(value) <= with_default 0 (FMap.find param.(from) (tokens state)) /\
+  (param.(from) <> ctx.(ctx_from) ->
+    param.(value) <= with_default 0 (FMap.find (param.(from), ctx.(ctx_from)) (allowances state)))
+    <-> exists new_state new_acts, receive chain ctx state (Some (msg_transfer param)) = Some (new_state, new_acts).
+Proof.
+  split.
+  - intros (amount_zero & enough_balance & enough_allowance).
+    (*do 2 eexists.
+    receive_simpl.*)
+    unfold receive.
+    apply Z.ltb_ge in amount_zero.
+    rewrite amount_zero.
+    cbn.
+    destruct_match eqn:allowances_eq;
+    destruct_match eqn:sender_from_eqb in allowances_eq; try congruence;
+    try destruct_match eqn:enough_allowance_check in allowances_eq; try congruence;
+    try destruct_match eqn:new_balance;
+    try destruct_match eqn:enough_balance_check in new_balance; try congruence.
+    + (* case no contradictions *)
+      inversion_clear allowances_eq.
+      now inversion_clear new_balance.
+    + (* enough balances contradiction *)
+      receive_simpl.
+      apply N.ltb_lt in enough_balance_check.
+      now apply N.le_ngt in enough_balance.
+    + (* case: no contradictions *)
+      inversion_clear allowances_eq.
+      now inversion_clear new_balance.
+    + (* enough balances contradiction *)
+      receive_simpl.
+      apply N.ltb_lt in enough_balance_check.
+      now apply N.le_ngt in enough_balance.
+    + (* enough allowance contradiction *)
+      receive_simpl.
+      apply N.ltb_lt in enough_allowance_check.
+      destruct (address_eqb_spec ctx.(ctx_from) param.(from)) as [| sender_from_ne]; try discriminate.
+      now apply not_eq_sym, enough_allowance, N.le_ngt in sender_from_ne.
+  - intros (new_state & new_acts & receive_some).
+    receive_simpl.
+    split; try now apply Z.ltb_ge in ctx_amount_zero.
+    clear ctx_amount_zero g0.
+    rename H1 into enough_balance.
+    apply N.ltb_ge in enough_balance.
+    rename H into allowance_check.
+    destruct_match eqn:sender_from_eqb in allowance_check;
+      destruct (address_eqb_spec ctx.(ctx_from) param.(from)) as
+        [send_from_eq | sender_from_ne]; try discriminate.
+    + (* sender = from *)
+      now split.
+    + (* sender <> from *)
+      destruct_match eqn:enough_allowance in allowance_check; try congruence.
+      receive_simpl.
+      now apply N.ltb_ge in enough_allowance.
+Qed.
+
+
+
+(* ------------------- Approve correct ------------------- *)
+
+(* try_approve correctly sets allowance of (<sender>, <spender>) to <value_> *)
+Lemma try_approve_allowance_correct : forall prev_state new_state chain ctx new_acts param,
+  receive chain ctx prev_state (Some (msg_approve param)) = Some (new_state, new_acts) ->
+    FMap.find (ctx.(ctx_from), param.(spender)) (allowances new_state) = Some param.(value_).
+Proof.
+  intros * receive_some.
+  receive_simpl.
+  clear H ctx_amount_zero.
+  cbn.
+  now rewrite FMap.find_add.
+Qed.
+
+(* try_approve does not produce any new actions *)
+Lemma try_approve_new_acts_correct : forall prev_state new_state chain ctx new_acts param,
+  receive chain ctx prev_state (Some (msg_approve param)) = Some (new_state, new_acts) ->
+    new_acts = [].
+Proof.
+  intros * receive_some.
+  receive_simpl.
+Qed.
+
+(* try_approve does not change allowances map of other addresses *)
+Lemma try_approve_preserves_other_allowances : forall prev_state new_state chain ctx new_acts param,
+  receive chain ctx prev_state (Some (msg_approve param)) = Some (new_state, new_acts) ->
+    forall allowance_key, allowance_key <> (ctx.(ctx_from), param.(spender)) ->
+      FMap.find allowance_key (allowances prev_state) = FMap.find allowance_key (allowances new_state).
+Proof.
+  intros * receive_some allowance_key allowance_key_ne.
+  receive_simpl.
+  clear H ctx_amount_zero.
+  cbn.
+  now rewrite FMap.find_add_ne.
+Qed.
+
+(* try_approve does not change total supply of tokens *)
+Lemma try_approve_preserves_total_supply : forall prev_state new_state chain ctx new_acts param,
+  receive chain ctx prev_state (Some (msg_approve param)) = Some (new_state, new_acts) ->
+    total_supply prev_state = total_supply new_state.
+Proof.
+  intros * receive_some.
+  now receive_simpl.
+Qed.
+
+(* try_approve does not change balances *)
+Lemma try_approve_preserves_balances : forall prev_state new_state chain ctx new_acts param,
+  receive chain ctx prev_state (Some (msg_approve param)) = Some (new_state, new_acts) ->
+    tokens prev_state = tokens new_state.
+Proof.
+  intros * receive_some.
+  now receive_simpl.
+Qed.
+
+(* If the requirements are met then then receive on approve msg must succeed and
+    if receive on approve msg succeeds then requirements must hold *)
+Lemma try_approve_is_some : forall state chain ctx param,
+  (ctx_amount ctx <= 0)%Z /\
+  (with_default 0 (FMap.find (ctx.(ctx_from), param.(spender)) (allowances state)) = 0 \/ param.(value_) = 0)
+    <-> exists new_state new_acts, receive chain ctx state (Some (msg_approve param)) = Some (new_state, new_acts).
+Proof.
+  split.
+  - intros (amount_zero & safe_approval).
+    do 2 eexists.
+    receive_simpl.
+    apply Z.ltb_ge in amount_zero.
+    rewrite amount_zero.
+    destruct_match eqn:safe_approval_check; eauto.
+    receive_simpl.
+    apply andb_prop in safe_approval_check as
+      (?%N.ltb_lt & ?%N.ltb_lt).
+    now destruct safe_approval.
+  - intros (new_state & new_acts & receive_some).
+    receive_simpl.
+    split; try now apply Z.ltb_ge in ctx_amount_zero.
+    rename H into safe_approval.
+    now apply andb_false_iff in safe_approval as [?%N.ltb_ge | ?%N.ltb_ge].
+Qed.
+
+
+
+(* ------------------- Burn or mint correct ------------------- *)
+
+(* try_mint_or_burn correctly mints/burns <amount> from/to <target> *)
+Lemma try_mint_or_burn_balance_correct : forall prev_state new_state chain ctx new_acts param,
+  receive chain ctx prev_state (Some (msg_mint_or_burn param)) = Some (new_state, new_acts) ->
+    (Z.of_N (with_default 0%N (FMap.find param.(target) (tokens prev_state))) + param.(quantity) =
+    Z.of_N (with_default 0%N (FMap.find param.(target) (tokens new_state))))%Z.
+Proof.
+  intros * receive_some.
+  receive_simpl.
+  rename H0 into enough_tokens.
+  clear ctx_amount_zero H.
+  rewrite Z.ltb_ge in enough_tokens.
+  cbn.
+  rewrite FMap.find_add.
+  cbn.
+  now rewrite Z2N.id.
+Qed.
+
+(* try_mint_or_burn correctly updates total_supply *)
+Lemma try_mint_or_burn_total_supply_correct : forall prev_state new_state chain ctx new_acts param,
+  with_default 0 (FMap.find param.(target) (tokens prev_state)) <= total_supply prev_state ->
+  receive chain ctx prev_state (Some (msg_mint_or_burn param)) = Some (new_state, new_acts) ->
+    (Z.of_N prev_state.(total_supply) + param.(quantity) =
+    Z.of_N new_state.(total_supply))%Z.
+Proof.
+  intros * balance_le_total_supply receive_some.
+  receive_simpl.
+  rename H0 into enough_tokens.
+  clear ctx_amount_zero H.
+  rewrite Z.ltb_ge in enough_tokens.
+  cbn.
+  rewrite N2Z.inj_abs_N, Z.abs_eq; auto.
+  eapply Z.le_trans; try apply enough_tokens.
+  now apply Zplus_le_compat_r, N2Z.inj_le.
+Qed.
+
+
+(* try_mint_or_burn produces no new actions *)
+Lemma try_mint_or_burn_new_acts_correct : forall prev_state new_state chain ctx new_acts param,
+  receive chain ctx prev_state (Some (msg_mint_or_burn param)) = Some (new_state, new_acts) ->
+    new_acts = [].
+Proof.
+  intros.
+  receive_simpl.
+Qed.
+
+(* try_mint_or_burn only modifies the <target> balance *)
+Lemma try_mint_or_burn_preserves_other_balances : forall prev_state new_state chain ctx new_acts param,
+  receive chain ctx prev_state (Some (msg_mint_or_burn param)) = Some (new_state, new_acts) ->
+    forall account, account <> param.(target) ->
+      FMap.find account (tokens prev_state) = FMap.find account (tokens new_state).
+Proof.
+  intros * receive_some account account_not_target.
+  receive_simpl.
+  cbn.
+  rewrite FMap.find_add_ne; auto.
+Qed.
+
+(* try_mint_or_burn does not change allowances *)
+Lemma try_mint_or_burn_preserves_allowances : forall prev_state new_state chain ctx new_acts param,
+  receive chain ctx prev_state (Some (msg_mint_or_burn param)) = Some (new_state, new_acts) ->
+      allowances prev_state = allowances new_state.
+Proof.
+  intros * receive_some.
+  now receive_simpl.
+Qed.
+
+(* If the requirements are met then then receive on mint_or_burn msg must succeed and
+    if receive on mint_or_burn msg succeeds then requirements must hold *)
+Lemma try_mint_or_burn_is_some : forall state chain ctx param,
+  (ctx_amount ctx <= 0)%Z /\
+  ctx.(ctx_from) = state.(admin) /\
+  (0 <= Z.of_N (with_default 0%N (FMap.find param.(target) (tokens state))) + param.(quantity))%Z
+    <-> exists new_state new_acts, receive chain ctx state (Some (msg_mint_or_burn param)) = Some (new_state, new_acts).
+Proof.
+  split.
+  - intros (amount_zero & from_admin & enough_balance).
+    do 2 eexists.
+    receive_simpl.
+    apply Z.ltb_ge in amount_zero.
+    rewrite amount_zero.
+    destruct_address_eq; try congruence.
+    clear e from_admin. cbn.
+    destruct_match eqn:enough_balance_check; eauto.
+    receive_simpl.
+    now apply Z.ltb_lt in enough_balance_check.
+  - intros (new_state & new_acts & receive_some).
+    receive_simpl.
+    split; try now apply Z.ltb_ge in ctx_amount_zero.
+    split; try now destruct_address_eq.
+    now apply Z.ltb_ge.
+Qed.
+
+
+
+(* ------------------- Get allowance correct ------------------- *)
+
+(* try_get_allowance produces a callback to the correct contract with
+    the requested allowance, the call should carry no balance *)
+Lemma try_get_allowance_new_acts_correct : forall prev_state new_state chain ctx new_acts param,
+  receive chain ctx prev_state (Some (msg_get_allowance param)) = Some (new_state, new_acts) ->
+    new_acts = [
+      act_call ctx.(ctx_from) 0%Z (serialize
+        (receive_allowance (with_default 0 (FMap.find param.(request) (allowances prev_state)))))
+    ].
+Proof.
+  intros * receive_some.
+  now receive_simpl.
+Qed.
+
+(* try_get_allowance does not modify state *)
+Lemma try_get_allowance_preserves_state : forall prev_state new_state chain ctx new_acts param,
+  receive chain ctx prev_state (Some (msg_get_allowance param)) = Some (new_state, new_acts) ->
+    prev_state = new_state.
+Proof.
+  intros * receive_some.
+  now receive_simpl.
+Qed.
+
+(* If the requirements are met then then receive on get_allowance msg must succeed and
+    if receive on get_allowance msg succeeds then requirements must hold *)
+Lemma try_get_allowance_is_some : forall prev_state chain ctx param,
+  (ctx_amount ctx <= 0)%Z <->
+  exists new_state new_acts, receive chain ctx prev_state (Some (msg_get_allowance param)) = Some (new_state, new_acts).
+Proof.
+  split.
+  - intros amount_zero.
+    unfold receive.
+    apply Z.ltb_ge in amount_zero.
+    now rewrite amount_zero.
+  - intros (new_state & new_acts & receive_some).
+    receive_simpl.
+    now apply Z.ltb_ge in ctx_amount_zero.
+Qed.
+
+
+
+(* ------------------- Get balance correct ------------------- *)
+
+(* try_get_balance produces a callback to the correct contract with
+    the requested balance, the call should carry no balance *)
+Lemma try_get_balance_new_acts_correct : forall prev_state new_state chain ctx new_acts param,
+  receive chain ctx prev_state (Some (msg_get_balance param)) = Some (new_state, new_acts) ->
+    new_acts = [
+      act_call ctx.(ctx_from) 0%Z (serialize
+        (receive_balance_of (with_default 0 (FMap.find param.(owner_) (tokens prev_state)))))
+    ].
+Proof.
+  intros * receive_some.
+  now receive_simpl.
+Qed.
+
+(* try_get_balance does not modify state *)
+Lemma try_get_balance_preserves_state : forall prev_state new_state chain ctx new_acts param,
+  receive chain ctx prev_state (Some (msg_get_balance param)) = Some (new_state, new_acts) ->
+    prev_state = new_state.
+Proof.
+  intros * receive_some.
+  now receive_simpl.
+Qed.
+
+(* If the requirements are met then then receive on get_balance msg must succeed and
+    if receive on get_balance msg succeeds then requirements must hold *)
+Lemma try_get_balance_is_some : forall prev_state chain ctx param,
+  (ctx_amount ctx <= 0)%Z <->
+  exists new_state new_acts, receive chain ctx prev_state (Some (msg_get_balance param)) = Some (new_state, new_acts).
+Proof.
+  split.
+  - intros amount_zero.
+    unfold receive.
+    apply Z.ltb_ge in amount_zero.
+    now rewrite amount_zero.
+  - intros (new_state & new_acts & receive_some).
+    receive_simpl.
+    now apply Z.ltb_ge in ctx_amount_zero.
+Qed.
+
+
+
+(* ------------------- Get total supply correct ------------------- *)
+
+(* try_get_total_supply produces a callback to the correct contract with
+    the tptal supply of tokens, the call should carry no balance *)
+Lemma try_get_total_supply_new_acts_correct : forall prev_state new_state chain ctx new_acts param,
+  receive chain ctx prev_state (Some (msg_get_total_supply param)) = Some (new_state, new_acts) ->
+    new_acts = [
+      act_call ctx.(ctx_from) 0%Z (serialize
+        (receive_total_supply prev_state.(total_supply)))
+    ].
+Proof.
+  intros * receive_some.
+  now receive_simpl.
+Qed.
+
+(* try_get_total_supply does not modify state *)
+Lemma try_get_total_supply_preserves_state : forall prev_state new_state chain ctx new_acts param,
+  receive chain ctx prev_state (Some (msg_get_total_supply param)) = Some (new_state, new_acts) ->
+    prev_state = new_state.
+Proof.
+  intros * receive_some.
+  now receive_simpl.
+Qed.
+
+(* If the requirements are met then then receive on get_total_supply msg must succeed and
+    if receive on get_total_supply msg succeeds then requirements must hold *)
+Lemma try_get_total_supply_is_some : forall prev_state chain ctx param,
+  (ctx_amount ctx <= 0)%Z <->
+  exists new_state new_acts, receive chain ctx prev_state (Some (msg_get_total_supply param)) = Some (new_state, new_acts).
+Proof.
+  split.
+  - intros amount_zero.
+    unfold receive.
+    apply Z.ltb_ge in amount_zero.
+    now rewrite amount_zero.
+  - intros (new_state & new_acts & receive_some).
+    receive_simpl.
+    now apply Z.ltb_ge in ctx_amount_zero.
+Qed.
+
+
+
+(* ------------------- Total supply / token balance facts ------------------- *)
+
+(* sum of all token balances *)
+Definition sum_balances state :=
+  sumN (fun '(k, v) => v) (FMap.elements (tokens state)).
+
+Lemma sum_balances_eq_total_supply : forall bstate caddr,
+  reachable bstate ->
+  env_contracts bstate caddr = Some (contract : WeakContract) ->
+  exists cstate,
+    contract_state bstate caddr = Some cstate
+    /\ total_supply cstate = sum_balances cstate.
+Proof.
+Admitted.
+
+Lemma token_balance_le_total_supply : forall bstate caddr,
+  reachable bstate ->
+  env_contracts bstate caddr = Some (contract : WeakContract) ->
+  exists cstate,
+    contract_state bstate caddr = Some cstate
+    /\ forall addr, with_default 0 (FMap.find addr (tokens cstate)) <= total_supply cstate.
+Proof.
+Admitted.
+
+
+
+
+
+(*
+  TODO
+    init correct
+    sum of balances eq total_supply
+    single token balance less than total supply
+*)
+
+
+
+
+End Theories.
 End LQTFA12.
